advancing in the proof

ver2/concrete_interpreter.v
@@ -27,25 +27,25 @@ Import Misc.
 Module ConcreteInterpreter.
 
 (* version operating on execution states *)
-Definition push_c (v : EVMWord) (st : state) : option state :=
+Definition push_c (v : EVMWord) (st : state) (ops : stack_op_instr_map) : option state :=
   let stk := get_stack_st st in
   match push v stk with
   | None => None
   | Some stk' => Some (set_stack_st st stk')
   end.
 
-Definition pop_c (st : state): option state := let stk := get_stack_st
+Definition pop_c (st : state) (ops : stack_op_instr_map): option state := let stk := get_stack_st
 st in match pop stk with | None => None | Some stk' => Some
 (set_stack_st st stk') end.
 
-Definition dup_c (k : nat) (st : state) : option state :=
+Definition dup_c (k : nat) (st : state) (ops : stack_op_instr_map) : option state :=
   let stk := get_stack_st st in
   match dup k stk with
   | None => None
   | Some stk' => Some (set_stack_st st stk')
   end.
 
-Definition swap_c (k : nat) (st : state) : option state :=
+Definition swap_c (k : nat) (st : state) (ops : stack_op_instr_map) : option state :=
   let stk := get_stack_st st in
   match swap k stk with
   | None => None
@@ -81,14 +81,14 @@ Definition sload (strg : storage) (key : EVMWord) := strg key.
 Definition sstore (strg : storage) (key : EVMWord) (value : EVMWord) :=
   fun key' => if (weqb key' key) then value else strg key'.
 
-Definition mload_c (st : state) : option state :=
+Definition mload_c (st : state) (ops : stack_op_instr_map) : option state :=
   match get_stack_st st with
   | offset::stk => let v := mload (get_memory_st st) offset in
                    let st' := set_stack_st st (v::stk) in
                    Some st'
   | _ => None end.
 
-Definition mstore8_c (st : state) : option state :=
+Definition mstore8_c (st : state) (ops : stack_op_instr_map) : option state :=
   match get_stack_st st with
   | offset::value::stk =>
       let mem := mstore8 (get_memory_st st) offset (split1 8 (EVMWordSize-8) value) in
@@ -97,7 +97,7 @@ Definition mstore8_c (st : state) : option state :=
       Some st''
   | _ => None end.
 
-Definition mstore_c (st : state) : option state :=
+Definition mstore_c (st : state) (ops : stack_op_instr_map) : option state :=
   match get_stack_st st with
   | offset::value::stk =>
       let mem := mstore (get_memory_st st) offset value in
@@ -105,7 +105,7 @@ Definition mstore_c (st : state) : option state :=
       let st'' := set_stack_st st' stk in Some st''
   | _ => None end.
 
-Definition sload_c (st : state) : option state :=
+Definition sload_c (st : state) (ops : stack_op_instr_map) : option state :=
   match get_stack_st st with
   | key::stk =>
       let v := sload (get_storage_st st) key in
@@ -113,7 +113,7 @@ Definition sload_c (st : state) : option state :=
       Some st'
   | _ => None end.
 
-Definition sstore_c (st : state) : option state :=
+Definition sstore_c (st : state) (ops : stack_op_instr_map) : option state :=
   match get_stack_st st with
   | key::value::stk =>
       let strg := sstore (get_storage_st st) key value in
@@ -123,7 +123,7 @@ Definition sstore_c (st : state) : option state :=
   | _ => None end.
 
 (* just return 0 for now *)
-Definition sha3_c (st : state) : option state :=
+Definition sha3_c (st : state) (ops : stack_op_instr_map) : option state :=
   match get_stack_st st with
   | offset::size::stk =>
       let f := get_keccak256_ctx (get_context_st st) in
@@ -133,7 +133,7 @@ Definition sha3_c (st : state) : option state :=
   | _ =>
 None end.
 
-Definition exec_stack_op_intsr_c (st : state) (ops : stack_op_instr_map) (label : stack_op_instr) : option state :=
+Definition exec_stack_op_intsr_c (label : stack_op_instr) (st : state) (ops : stack_op_instr_map)  : option state :=
   match (ops label) with
   | OpImp nb_args func _ =>
       let stk := get_stack_st st in
@@ -150,30 +150,30 @@ Definition exec_stack_op_intsr_c (st : state) (ops : stack_op_instr_map) (label 
   end.
 
 (* Concrete interpreter *)
-Definition evm_exec_instr (inst : instr) (st: state) (ops : stack_op_instr_map) : option state :=
+Definition evm_exec_instr_c (inst : instr) (st: state) (ops : stack_op_instr_map) : option state :=
   match inst with
-  | PUSH size v => push_c (NToWord EVMWordSize v) st
-  | POP => pop_c st
-  | DUP k => dup_c k st
-  | SWAP k => swap_c k st
-  | MLOAD => mload_c st
-  | MSTORE8 => mstore8_c st
-  | MSTORE => mstore_c st
-  | SLOAD => sload_c st
-  | SSTORE => sstore_c st
-  | SHA3 => sha3_c st
-  | KECCAK256 => sha3_c st
-  | OpInstr label => exec_stack_op_intsr_c st ops label
+  | PUSH size v => push_c (NToWord EVMWordSize v) st ops
+  | POP => pop_c st ops
+  | DUP k => dup_c k st ops
+  | SWAP k => swap_c k st ops
+  | MLOAD => mload_c st ops
+  | MSTORE8 => mstore8_c st ops
+  | MSTORE => mstore_c st ops
+  | SLOAD => sload_c st ops
+  | SSTORE => sstore_c st ops
+  | SHA3 => sha3_c st ops
+  | KECCAK256 => sha3_c st ops
+  | OpInstr label => exec_stack_op_intsr_c label st ops
   end.
 
                
-Fixpoint evm_exec_block (p : block) (st : state) (ops : stack_op_instr_map) : option state :=
+Fixpoint evm_exec_block_c (p : block) (st : state) (ops : stack_op_instr_map) : option state :=
   match p with
   | [] => Some st
   | instr::instrs' =>
-      match evm_exec_instr instr st ops with
+      match evm_exec_instr_c instr st ops with
       | None => None
-      | Some st' => evm_exec_block instrs' st' ops
+      | Some st' => evm_exec_block_c instrs' st' ops
       end
   end.
 
