ver2/symbolic_execution_soundness.v
@@ -1,0 +1,169 @@
+Require Import Arith.
+Require Import Nat.
+Require Import Bool.
+Require Import bbv.Word.
+Require Import Coq.NArith.NArith.
+Require Import List.
+Import ListNotations.
+
+Require Import FORVES.constants.
+Import Constants.
+
+Require Import FORVES.program.
+Import Program.
+
+Require Import FORVES.execution_state.
+Import ExecutionState.
+
+Require Import FORVES.stack_operation_instructions.
+Import StackOpInstrs.
+
+Require Import FORVES.misc.
+Import Misc.
+
+Require Import FORVES.symbolic_state.
+Import SymbolicState.
+
+Require Import FORVES.symbolic_execution.
+Import SymbolicExecution.
+
+Require Import FORVES.symbolic_execution.
+Import SymbolicExecution.
+
+Require Import FORVES.symbolic_state_eval.
+Import SymbolicStateEval.
+
+Require Import FORVES.flat_symbolic_state.
+Import FlatSymbolicState.
+
+Require Import FORVES.concrete_interpreter.
+Import ConcreteInterpreter.
+
+Module SymbolicExecutionSoundness.
+
+Definition eq_con_sym (st: state) (sst: sstate) (ops: stack_op_instr_map) : Prop :=
+  exists (st': state),
+    eval_sstate st sst ops = Some st' /\
+    eq_execution_states st st'.
+  
+  
+Definition snd_state_transformer ( tr : state -> stack_op_instr_map -> option state ) (symtr : sstate ->  stack_op_instr_map -> option sstate )  : Prop :=
+  forall (sst sst': sstate) (ops : stack_op_instr_map),
+    symtr sst ops = Some sst' ->
+    forall (st: state),
+      eq_con_sym st sst ops ->
+        exists (st': state), tr st ops = Some st' /\ eq_con_sym st' sst' ops.
+
+
+
+Lemma push_snd:
+  forall w, snd_state_transformer (push_c w) (push_s w).       
+Proof.
+Admitted.
+
+Lemma pop_snd:
+  snd_state_transformer pop_c pop_s.       
+Proof.
+Admitted.
+
+Lemma dup_snd:
+  forall k, snd_state_transformer (dup_c k) (dup_s k).       
+Proof.
+Admitted.
+
+Lemma swap_snd:
+  forall k, snd_state_transformer (swap_c k) (swap_s k).
+Proof.
+Admitted.
+
+Lemma sload_snd:
+  snd_state_transformer sload_c sload_s.
+Proof.
+Admitted.
+
+Lemma sstore_snd:
+  snd_state_transformer sstore_c sstore_s.
+Proof.
+Admitted.
+
+Lemma mload_snd:
+  snd_state_transformer mload_c mload_s.
+Proof.
+Admitted.
+
+Lemma mstore8_snd:
+  snd_state_transformer mstore8_c mstore8_s.
+Proof.
+Admitted.
+
+Lemma mstore_snd:
+  snd_state_transformer mstore_c mstore_s.
+Proof.
+Admitted.
+
+Lemma sha3_snd:
+  snd_state_transformer sha3_c sha3_s.
+Proof.
+Admitted.
+
+Lemma exec_stack_op_intsr_snd:
+  forall label, snd_state_transformer (exec_stack_op_intsr_c label) (exec_stack_op_intsr_s label).
+Proof.
+Admitted.
+
+
+Lemma evm_exec_instr_snd:
+  forall (i : instr),
+    snd_state_transformer (evm_exec_instr_c i) (evm_exec_instr_s i).
+Proof.
+  destruct i.
+  - unfold evm_exec_instr_c. unfold evm_exec_instr_s. apply push_snd.
+  - unfold evm_exec_instr_c. unfold evm_exec_instr_s. apply pop_snd.
+  - unfold evm_exec_instr_c. unfold evm_exec_instr_s. apply dup_snd.
+  - unfold evm_exec_instr_c. unfold evm_exec_instr_s. apply swap_snd.
+  - unfold evm_exec_instr_c. unfold evm_exec_instr_s. apply mload_snd.
+  - unfold evm_exec_instr_c. unfold evm_exec_instr_s. apply mstore_snd.
+  - unfold evm_exec_instr_c. unfold evm_exec_instr_s. apply mstore8_snd.
+  - unfold evm_exec_instr_c. unfold evm_exec_instr_s. apply sload_snd.
+  - unfold evm_exec_instr_c. unfold evm_exec_instr_s. apply sstore_snd.
+  - unfold evm_exec_instr_c. unfold evm_exec_instr_s. apply sha3_snd.
+  - unfold evm_exec_instr_c. unfold evm_exec_instr_s. apply sha3_snd.
+  - unfold evm_exec_instr_c. unfold evm_exec_instr_s. apply exec_stack_op_intsr_snd.
+Qed.
+
+  
+Lemma evm_exec_block_snd:
+  forall (p : block),
+    snd_state_transformer (evm_exec_block_c p) (evm_exec_block_s p).
+Proof.
+  unfold snd_state_transformer.
+  induction p as [| i p' IHp'].
+  - intros. simpl. exists st. split.
+    + reflexivity.
+    + injection H as H1. rewrite <- H1. apply H0.
+  - intros. unfold evm_exec_block_s in H. fold evm_exec_block_s in H.
+    destruct (evm_exec_instr_s i sst ops) eqn:E.
+    + apply evm_exec_instr_snd in E as E0. destruct E0 with (st:=st). apply H0.
+      apply IHp' with (st:=x) in H.
+      * destruct H. exists x0. split.
+        ** unfold evm_exec_block_c. destruct H1. rewrite H1. fold evm_exec_block_c. destruct H. apply H.
+        ** destruct H. apply H2.
+      * destruct H1. apply H2.
+    + discriminate H.
+Qed.
+
+
+Theorem symbolic_exec_snd:
+  forall (p : block) (instk_height : nat) (sst : sstate) (ops : stack_op_instr_map),
+    evm_sym_exec p instk_height ops = Some sst -> 
+    forall (st : state), 
+      length (get_stack_st st) = instk_height -> 
+      exists (st': state),
+        evm_exec_block_c p st ops = Some st' /\
+          eq_con_sym st' sst ops. 
+Proof.
+  Admitted.
+
+Check symbolic_exec_snd.
+  
+End SymbolicExecutionSoundness.
